examples/ghc/lib/Constants.v
@@ -14,39 +14,28 @@ Require Coq.Program.Wf.
 
 Require GHC.Nat.
 
-(* Converted imports: *)
-
-Require GHC.Num.
-Import GHC.Num.Notations.
+(* No imports to convert. *)
 
 (* No type declarations to convert. *)
 
 (* Converted value declarations: *)
 
-Definition wORD64_SIZE : nat :=
-  #8.
+Axiom wORD64_SIZE : nat.
 
-Definition tARGET_MAX_CHAR : nat :=
-  #1114111.
+Axiom tARGET_MAX_CHAR : nat.
 
-Definition mAX_TUPLE_SIZE : nat :=
-  #62.
+Axiom mAX_TUPLE_SIZE : nat.
 
-Definition mAX_SUM_SIZE : nat :=
-  #62.
+Axiom mAX_SUM_SIZE : nat.
 
-Definition mAX_SOLVER_ITERATIONS : nat :=
-  #4.
+Axiom mAX_SOLVER_ITERATIONS : nat.
 
-Definition mAX_REDUCTION_DEPTH : nat :=
-  #200.
+Axiom mAX_REDUCTION_DEPTH : nat.
 
-Definition mAX_CTUPLE_SIZE : nat :=
-  #62.
+Axiom mAX_CTUPLE_SIZE : nat.
 
-Definition fLOAT_SIZE : nat :=
-  #4.
+Axiom fLOAT_SIZE : nat.
 
 (* External variables:
-     nat GHC.Num.fromInteger
+     nat
 *)
